Given that T(n) represents the sum of the first $n$ terms, it can be expressed as:

$T(n) = a_1 + a_2 + ... + a_n$

$T(n) = (c_1 + c_2) + (2c_1 + c_2) + \ldots + (nc_1 + c_2)$

According to the book's analysis in Section 2.2, T(n) is a quadratic function, and we can express it as:

$T(n) = k_1 n^2 + k_2 n + k_3$

Now, let's determine the values of the constants $k_1$, $k_2$, and $k_3$.

1. For $n = 0$, we have $T(0) = 0$, which implies that $k_3 = 0$.

2. For $n = 1$, we find that $T(1) = c_1 + c_2$. Thus, we can express $k_1$ in terms of $c_1, c_2$, and $k2$
as follows: $k_1 = c_1 + c_2 - k_2$.

3. For $n = 2$, we get $T(2) = 3c_1 + 2c_2$, which can be equated to $4k_1 + 2k_2$. This allows us to express 
$k_2$ in terms of $c_1$ and $c_2$ as follows: $k_2 = 1/2(c_1 + 2c_2)$, and we can use the previously determined value
of $k_1$.

Therefore, we have found the expressions for $k_1$ and $k_2$:

$k_1 = c_1 + c_2 - k_2$
$k_2 = \frac{1}{2}(c_1 + 2c_2)$

Thus, $T(n)$ can be expressed as:

$T(n) = \frac{1}{2} c_1 n^2 + \frac{1}{2} (c_1 + 2c_2) n$

Now, to prove this by induction:

Base case $(n = 1)$: $T(1) = \frac{1}{2} c_1 + \frac{1}{2} (c_1 + 2c_2) = c_1 + c_2$, which is true.

Inductive step $(n = k+1)$:

Assume that $T(k) = \frac{1}{2} c_1 k^2 + \frac{1}{2} (c_1 + 2c_2) k$ is true for some positive integer $k$.

We want to prove that $T(k+1) = \frac{1}{2} c_1 (k+1)^2 + \frac{1}{2} (c_1 + 2c_2) (k+1)$.

Starting with $T(k+1)$, we have:

$T(k+1) = T(k) + c_1(k+1) + c_2$
$T(k+1) = [\frac{1}{2} c_1 k^2 + \frac{1}{2} (c_1 + 2c_2) k] + c_1(k+1) + c_2$

Now, let's simplify this expression:

$T(k+1) = 1/2 c_1 k^2 + 1/2 (c_1 + 2c_2) k + c_1(k+1) + c_2$
$T(k+1) = 1/2 c_1 (k^2 + 2k + 1) + (1/2 c_1 + c_2)(k+1)$

Using the identity $(k^2 + 2k + 1) = (k+1)^2$, we can simplify further:

$T(k+1) = 1/2 c_1 (k+1)^2 + (1/2 c_1 + c_2)(k+1)$

Thus, we have successfully proven that $T(n) = 1/2 c_1 n^2 + 1/2 (c_1 + 2c_2) n$ by induction.
